nix/shell/default.nix
@@ -1,23 +1,25 @@
 {
-  perSystem = {pkgs, ...}: {
-    devShells.default = pkgs.mkShell {
-      packages = with pkgs; [
-        # Nix
-        nixd
-        statix
-        deadnix
-        nixfmt
-        alejandra
+  perSystem =
+    { pkgs, ... }:
+    {
+      devShells.default = pkgs.mkShell {
+        packages = with pkgs; [
+          # Nix
+          nixd
+          statix
+          deadnix
+          nixfmt
+          alejandra
 
-        # Rust
-        cargo
-        rustc
-        rust-analyzer
-        bacon
+          # Rust
+          cargo
+          rustc
+          rust-analyzer
+          bacon
 
-        # Lean
-        lean4
-      ];
+          # Lean
+          lean4
+        ];
+      };
     };
-  };
 }
