templates/rust/flake.nix
@@ -3,69 +3,72 @@
 {
   description = "Rust project";
 
-  outputs = inputs @ {
-    flake-parts,
-    crane,
-    advisory-db,
-    lean4-nix,
-    ...
-  }:
-    flake-parts.lib.mkFlake {inherit inputs;} {
-      perSystem = {
-        # NOTE: This packages is only used to construct the common argument for
-        # crane; the actual `pkgs` used in the other Nix modules are defined
-        # below
-        pkgs,
-        system,
-        ...
-      }: let
-        craneLib = crane.mkLib pkgs;
-        # Common arguments can be set here to avoid repeating them later
-        # NOTE: changes here will rebuild all dependency crates
-        src = craneLib.cleanCargoSource ./.;
-        commonArgs = {
-          inherit src;
-          strictDeps = true;
+  outputs =
+    inputs@{
+      flake-parts,
+      crane,
+      advisory-db,
+      lean4-nix,
+      ...
+    }:
+    flake-parts.lib.mkFlake { inherit inputs; } {
+      perSystem =
+        {
+          # NOTE: This packages is only used to construct the common argument for
+          # crane; the actual `pkgs` used in the other Nix modules are defined
+          # below
+          pkgs,
+          system,
+          ...
+        }:
+        let
+          craneLib = crane.mkLib pkgs;
+          # Common arguments can be set here to avoid repeating them later
+          # NOTE: changes here will rebuild all dependency crates
+          src = craneLib.cleanCargoSource ./.;
+          commonArgs = {
+            inherit src;
+            strictDeps = true;
 
-          buildInputs = pkgs.lib.optionals pkgs.stdenv.isDarwin [
-            pkgs.libiconv
-          ];
+            buildInputs = pkgs.lib.optionals pkgs.stdenv.isDarwin [
+              pkgs.libiconv
+            ];
 
-          nativeBuildInputs = [
-            pkgs.pkg-config
-          ];
-        };
-
-        cargoArtifacts = craneLib.buildDepsOnly commonArgs;
-
-        charonToolchain =
-          inputs.aeneas.inputs.charon.packages.${system}.rustToolchain;
-
-        # Used to build Lean packages
-        lake2nix = pkgs.callPackage lean4-nix.lake {};
-      in {
-        _module.args = {
-          inherit
-            craneLib
-            cargoArtifacts
-            commonArgs
-            src
-            charonToolchain
-            advisory-db
-            lake2nix
-            ;
-
-          # NOTE: This is where overlays, and other such modifications to the
-          # general shared packages list.
-          pkgs = import inputs.nixpkgs {
-            inherit system;
-            overlays = [
-              inputs.rust-overlay.overlays.default
-              (inputs.lean4-nix.readToolchainFile ./proofs/lean-toolchain)
+            nativeBuildInputs = [
+              pkgs.pkg-config
             ];
           };
+
+          cargoArtifacts = craneLib.buildDepsOnly commonArgs;
+
+          charonToolchain = inputs.aeneas.inputs.charon.packages.${system}.rustToolchain;
+
+          # Used to build Lean packages
+          lake2nix = pkgs.callPackage lean4-nix.lake { };
+        in
+        {
+          _module.args = {
+            inherit
+              craneLib
+              cargoArtifacts
+              commonArgs
+              src
+              charonToolchain
+              advisory-db
+              lake2nix
+              ;
+
+            # NOTE: This is where overlays, and other such modifications to the
+            # general shared packages list.
+            pkgs = import inputs.nixpkgs {
+              inherit system;
+              overlays = [
+                inputs.rust-overlay.overlays.default
+                (inputs.lean4-nix.readToolchainFile ./proofs/lean-toolchain)
+              ];
+            };
+          };
         };
-      };
       imports = [
         ./nix/shell
         ./nix/pkgs
