templates/rust/nix/shell/default.nix
@@ -1,43 +1,46 @@
 {
-  perSystem = {
-    pkgs,
-    craneLib,
-    inputs',
-    self',
-    ...
-  }: let
-    valeConfigured = pkgs.callPackage ./vale {};
+  perSystem =
+    {
+      pkgs,
+      craneLib,
+      inputs',
+      self',
+      ...
+    }:
+    let
+      valeConfigured = pkgs.callPackage ./vale { };
 
-    # Packages from this flake
-    leanTranslation = self'.packages.lean-translation;
-    aeneasLib = self'.packages.aeneas-lean-backend;
-  in {
-    devShells.default = craneLib.devShell {
-      packages = with pkgs; [
-        # Nix
-        nixd
-        statix
-        deadnix
-        alejandra
+      # Packages from this flake
+      leanTranslation = self'.packages.lean-translation;
+      aeneasLib = self'.packages.aeneas-lean-backend;
+    in
+    {
+      devShells.default = craneLib.devShell {
+        packages = with pkgs; [
+          # Nix
+          nixd
+          statix
+          deadnix
+          alejandra
 
-        # Rust
-        cargo-audit
-        cargo-expand
-        cargo-nextest
-        rust-analyzer
-        cargo-wizard
-        bacon
+          # Rust
+          cargo-audit
+          cargo-expand
+          cargo-nextest
+          rust-analyzer
+          cargo-wizard
+          bacon
 
-        # Prose
-        valeConfigured
+          # Prose
+          valeConfigured
 
-        # Theorem proving
-        inputs'.aeneas.packages.aeneas
-        lean4
-      ];
+          # Theorem proving
+          inputs'.aeneas.packages.aeneas
+          lean4
+        ];
 
-      LEAN_SRC_PATH = "${leanTranslation}/lib/lean:${aeneasLib}/lib/lean";
-      LEAN_PATH = "${leanTranslation}/lib/lean:${aeneasLib}/lib/lean";
+        LEAN_SRC_PATH = "${leanTranslation}/lib/lean:${aeneasLib}/lib/lean";
+        LEAN_PATH = "${leanTranslation}/lib/lean:${aeneasLib}/lib/lean";
+      };
     };
-  };
 }
